\begin{syntax}
  logic-type-decl ::= "logic" "type" logic-type = logic-type-def ";"  
  \
  logic-type-def ::= record-type | sum-type ; 
  \
  record-type ::= "{" type-expr id ( ";" type-expr id)* ";"? "}" 
  \
  sum-type ::= "|"? constructor ( "|" constructor)* 
  \
  constructor ::= id ; constant constructor
  | id "of" type-expr ; non-constant constructor
  \
  type-expr ::= type-expr ("*" type-expr)+ ; product type 
  \
  term ::= term "." id ; record field access
  | "\match" term ";" match-cases ; pattern-matching
  | "(" term ("," term)+ ")" ; tuples
  | "\let" "(" id (, id)+ ")" "=" term ";" term ; \experimental
  \
  match-cases ::= "|"? match-case ("|" match-case)* 
  \
  match-case ::= pattern ":" term
  \
  pattern ::= term ; see semantic conditions
\end{syntax}